EffectSSA/ProofSketch/Notation/Reduce.lean
@@ -1,5 +1,7 @@
 module
 
+public import EffectSSA.ProofSketch.Denote
+
 /-!
 # Reduction Semantics
 -/
@@ -36,16 +38,6 @@ inductive TReducesTo {α} [Reduce α] : α → α → Prop where
   | step {x y z} : ReducesTo x y → TReducesTo y z → TReducesTo x z
 scoped infixl:arg " ⟹+ " => TReducesTo
 
-class BReduce (α : Type) (β : outParam Type) extends Reduce α where
-  /-- Type `β` can be seen as a subset of states in `α` which describe value. -/
-  stateOfValue : β → α
-  /-- Values ought to be terminal, i.e, may not reduce further. -/
-  terminal_value : ∀ (b : β) (y : α), ¬(stateOfValue b ⟹ y) := by grind
-
-@[grind] def BReducesTo {α β} [BReduce α β] : α → β → Prop :=
-  fun x y => x ⟹+ (BReduce.stateOfValue y)
-scoped infixl:50 " ⇓ " => BReducesTo
-
 namespace TReducesTo
 variable {α} [Reduce α] {x y z : α}
 
@@ -64,4 +56,69 @@ instance : Trans (α:=α) (· ⟹+ ·) (· ⟹ ·) (· ⟹+ ·) where trans := b
 instance : Trans (α:=α) (· ⟹ ·) (· ⟹+ ·) (· ⟹+ ·) where trans := by grind
 
 end TReducesTo
+
+/-! ## Transitive, Reflexive Closure -/
+section Closure
+
+/--
+`x ⟹* y` holds when `x` reduces to `y` in zero or more steps.
+
+That is, `⟹*` is the transitive, reflexive closure of `⟹`.
+-/
+@[grind, grind cases]
+inductive TRReducesTo {α} [Reduce α] : α → α → Prop where
+  | refl {x} : TRReducesTo x x
+  | step {x y z} : ReducesTo x y → TRReducesTo y z → TRReducesTo x z
+scoped infixl:arg " ⟹* " => TRReducesTo
+
+namespace TRReducesTo
+variable {α} [Reduce α] {x y z : α}
+
+attribute [grind .] refl
+@[grind ., grind →] theorem ofReduce (h : x ⟹ y) : x ⟹* y := step h refl
+
+@[grind →] theorem trans : x ⟹* y → y ⟹* z → x ⟹* z := by
+  intro h₁ h₂
+  induction h₁
+  · grind
+  · apply step
+    · assumption
+    · grind
+
+instance : Trans (α:=α) (· ⟹* ·) (· ⟹* ·) (· ⟹* ·) where trans := by grind
+instance : Trans (α:=α) (· ⟹* ·) (· ⟹ ·) (· ⟹* ·) where trans := by grind
+instance : Trans (α:=α) (· ⟹ ·) (· ⟹* ·) (· ⟹* ·) where trans := by grind
+
+end TRReducesTo
+
+/-! ## Big-step reduction -/
+section BReduce
+
+class BReduce (α : Type) (β : outParam Type) extends Reduce α where
+  /-- Type `β` can be seen as a subset of states in `α` which describe value. -/
+  stateOfValue : β → α
+  /-- Values ought to be terminal, i.e, may not reduce further. -/
+  terminal_value : ∀ (b : β) (y : α), ¬(stateOfValue b ⟹ y) := by grind
+open BReduce
+
+@[grind, expose] def BReducesTo {α β} [BReduce α β] : α → β → Prop :=
+  fun x y => x ⟹* (stateOfValue y)
+scoped infixl:50 " ⇓ " => BReducesTo
+
+/--
+If a type has a `BReduce` instance into values of type `β`,
+this induces a denotation into a predicate over `β`.
+-/
+instance (priority := low) [BReduce α β] : Denote α (β → Prop) where
+  denote := fun a b => a ⇓ b
+
+section Lemma
+
+attribute [grind] BReduce.stateOfValue
+
+@[grind =] theorem bReducesTo_iff [BReduce α β] {x : α} {y : β} :
+  x ⇓ y ↔ x ⟹* (stateOfValue y) := by rfl
+
+end Lemma
+end BReduce
 end Closure
